examples/heapsort/Heapsort0.v
@@ -1,0 +1,38 @@
+Require Import Coqlib.
+Require Import ImpPrelude.
+Require Import STS.
+Require Import Behavior.
+Require Import ModSem.
+Require Import Skeleton.
+Require Import PCM.
+Require Import HoareDef.
+Require Import ProofMode.
+Require Import STB.
+Require Import HeapsortHeader.
+Require Import heapsort.
+Require Import ConvC2ITree.
+
+Definition globenv := Clight.globalenv prog.
+Definition create_body : list Values.val -> itree Es Values.val  := decomp_func globenv f_create.
+Definition heapify_body : list Values.val -> itree Es Values.val := decomp_func globenv f_heapify.
+Definition heapsort_body : list Values.val -> itree Es Values.val  := decomp_func globenv f_heapsort.
+
+Definition HeapsortSbtb :=
+  [("create",  cfunU create_body);
+   ("heapify",  cfunU heapify_body);
+   ("heapsort", cfunU heapsort_body)
+  ].
+
+Definition HeapsortSem : ModSem.t :=
+  {|
+    ModSem.fnsems := HeapsortSbtb;
+    ModSem.mn := "Heapsort";
+    ModSem.initial_st := tt↑;
+  |}.
+
+Definition Heapsort : Mod.t :=
+  {|
+    Mod.get_modsem := fun _ => HeapsortSem;
+    Mod.sk := Sk.unit;
+  |}.
+
