examples/heapsort/Heapsort01proof.v
@@ -1,0 +1,37 @@
+Require Import Coqlib.
+Require Import ImpPrelude.
+Require Import STS.
+Require Import Behavior.
+Require Import ModSem.
+Require Import Skeleton.
+Require Import PCM.
+Require Import HoareDef.
+Require Import ProofMode.
+Require Import STB.
+Require Import HeapsortHeader.
+Require Import HeapsortProperties.
+Require Import Heapsort0 Heapsort1.
+Require Import HTactics ProofMode.
+Require Import SimModSem.
+Require Import Coq.Sorting.Sorted.
+
+Section SIMMODSEM.
+
+  Context `{Σ : GRA.t}.
+
+  Variable GlobalStb : Sk.t -> gname -> option fspec.
+  Hypothesis STBINCL : forall sk, stb_incl (to_stb SHeapsortStb) (GlobalStb sk).
+  Hint Unfold SHeapsortStb : stb.
+
+  Definition wf : _ -> Any.t * Any.t -> Prop :=
+    @mk_wf
+      _
+      unit
+      (fun _ st_src st_tgt => True)%I.
+
+  
+
+  Theorem correct : refines2 [Heapsort0.Heapsort] [Heapsort1.Heapsort_to0 GlobalStb].
+  Proof.
+  Admitted.
+End SIMMODSEM.
