examples/heapsort/heapsort.v
@@ -1,0 +1,635 @@
+From Coq Require Import String List ZArith.
+From compcert Require Import Coqlib Integers Floats AST Ctypes Cop Clight Clightdefs.
+Import Clightdefs.ClightNotations.
+Local Open Scope Z_scope.
+Local Open Scope string_scope.
+Local Open Scope clight_scope.
+
+Module Info.
+  Definition version := "3.10".
+  Definition build_number := "".
+  Definition build_tag := "".
+  Definition build_branch := "".
+  Definition arch := "x86".
+  Definition model := "64".
+  Definition abi := "standard".
+  Definition bitsize := 64.
+  Definition big_endian := false.
+  Definition source_file := "heapsort.c".
+  Definition normalized := false.
+End Info.
+
+Definition ___builtin_ais_annot : ident := $"__builtin_ais_annot".
+Definition ___builtin_annot : ident := $"__builtin_annot".
+Definition ___builtin_annot_intval : ident := $"__builtin_annot_intval".
+Definition ___builtin_bswap : ident := $"__builtin_bswap".
+Definition ___builtin_bswap16 : ident := $"__builtin_bswap16".
+Definition ___builtin_bswap32 : ident := $"__builtin_bswap32".
+Definition ___builtin_bswap64 : ident := $"__builtin_bswap64".
+Definition ___builtin_clz : ident := $"__builtin_clz".
+Definition ___builtin_clzl : ident := $"__builtin_clzl".
+Definition ___builtin_clzll : ident := $"__builtin_clzll".
+Definition ___builtin_ctz : ident := $"__builtin_ctz".
+Definition ___builtin_ctzl : ident := $"__builtin_ctzl".
+Definition ___builtin_ctzll : ident := $"__builtin_ctzll".
+Definition ___builtin_debug : ident := $"__builtin_debug".
+Definition ___builtin_expect : ident := $"__builtin_expect".
+Definition ___builtin_fabs : ident := $"__builtin_fabs".
+Definition ___builtin_fabsf : ident := $"__builtin_fabsf".
+Definition ___builtin_fmadd : ident := $"__builtin_fmadd".
+Definition ___builtin_fmax : ident := $"__builtin_fmax".
+Definition ___builtin_fmin : ident := $"__builtin_fmin".
+Definition ___builtin_fmsub : ident := $"__builtin_fmsub".
+Definition ___builtin_fnmadd : ident := $"__builtin_fnmadd".
+Definition ___builtin_fnmsub : ident := $"__builtin_fnmsub".
+Definition ___builtin_fsqrt : ident := $"__builtin_fsqrt".
+Definition ___builtin_membar : ident := $"__builtin_membar".
+Definition ___builtin_memcpy_aligned : ident := $"__builtin_memcpy_aligned".
+Definition ___builtin_read16_reversed : ident := $"__builtin_read16_reversed".
+Definition ___builtin_read32_reversed : ident := $"__builtin_read32_reversed".
+Definition ___builtin_sel : ident := $"__builtin_sel".
+Definition ___builtin_sqrt : ident := $"__builtin_sqrt".
+Definition ___builtin_unreachable : ident := $"__builtin_unreachable".
+Definition ___builtin_va_arg : ident := $"__builtin_va_arg".
+Definition ___builtin_va_copy : ident := $"__builtin_va_copy".
+Definition ___builtin_va_end : ident := $"__builtin_va_end".
+Definition ___builtin_va_start : ident := $"__builtin_va_start".
+Definition ___builtin_write16_reversed : ident := $"__builtin_write16_reversed".
+Definition ___builtin_write32_reversed : ident := $"__builtin_write32_reversed".
+Definition ___compcert_i64_dtos : ident := $"__compcert_i64_dtos".
+Definition ___compcert_i64_dtou : ident := $"__compcert_i64_dtou".
+Definition ___compcert_i64_sar : ident := $"__compcert_i64_sar".
+Definition ___compcert_i64_sdiv : ident := $"__compcert_i64_sdiv".
+Definition ___compcert_i64_shl : ident := $"__compcert_i64_shl".
+Definition ___compcert_i64_shr : ident := $"__compcert_i64_shr".
+Definition ___compcert_i64_smod : ident := $"__compcert_i64_smod".
+Definition ___compcert_i64_smulh : ident := $"__compcert_i64_smulh".
+Definition ___compcert_i64_stod : ident := $"__compcert_i64_stod".
+Definition ___compcert_i64_stof : ident := $"__compcert_i64_stof".
+Definition ___compcert_i64_udiv : ident := $"__compcert_i64_udiv".
+Definition ___compcert_i64_umod : ident := $"__compcert_i64_umod".
+Definition ___compcert_i64_umulh : ident := $"__compcert_i64_umulh".
+Definition ___compcert_i64_utod : ident := $"__compcert_i64_utod".
+Definition ___compcert_i64_utof : ident := $"__compcert_i64_utof".
+Definition ___compcert_va_composite : ident := $"__compcert_va_composite".
+Definition ___compcert_va_float64 : ident := $"__compcert_va_float64".
+Definition ___compcert_va_int32 : ident := $"__compcert_va_int32".
+Definition ___compcert_va_int64 : ident := $"__compcert_va_int64".
+Definition _base : ident := $"base".
+Definition _child : ident := $"child".
+Definition _child_i : ident := $"child_i".
+Definition _create : ident := $"create".
+Definition _heapify : ident := $"heapify".
+Definition _heapsort : ident := $"heapsort".
+Definition _initval : ident := $"initval".
+Definition _k : ident := $"k".
+Definition _l : ident := $"l".
+Definition _main : ident := $"main".
+Definition _nmemb : ident := $"nmemb".
+Definition _par : ident := $"par".
+Definition _par_i : ident := $"par_i".
+Definition _tmp : ident := $"tmp".
+Definition _vbase : ident := $"vbase".
+Definition _t'1 : ident := 128%positive.
+Definition _t'2 : ident := 129%positive.
+Definition _t'3 : ident := 130%positive.
+
+Definition f_create := {|
+  fn_return := tvoid;
+  fn_callconv := cc_default;
+  fn_params := ((_base, (tptr tint)) :: (_nmemb, tulong) ::
+                (_initval, tulong) :: nil);
+  fn_vars := nil;
+  fn_temps := ((_par_i, tulong) :: (_child_i, tulong) ::
+               (_par, (tptr tint)) :: (_child, (tptr tint)) ::
+               (_tmp, tint) :: (_t'2, tint) :: (_t'1, tulong) :: nil);
+  fn_body :=
+(Ssequence
+  (Sset _par_i (Etempvar _initval tulong))
+  (Sloop
+    (Ssequence
+      (Ssequence
+        (Ssequence
+          (Sset _t'1
+            (Ecast
+              (Ebinop Omul (Etempvar _par_i tulong)
+                (Econst_int (Int.repr 2) tint) tulong) tulong))
+          (Sset _child_i (Etempvar _t'1 tulong)))
+        (Sifthenelse (Ebinop Ole (Etempvar _t'1 tulong)
+                       (Etempvar _nmemb tulong) tint)
+          Sskip
+          Sbreak))
+      (Ssequence
+        (Sset _child
+          (Ebinop Oadd (Etempvar _base (tptr tint))
+            (Etempvar _child_i tulong) (tptr tint)))
+        (Ssequence
+          (Ssequence
+            (Sifthenelse (Ebinop Olt (Etempvar _child_i tulong)
+                           (Etempvar _nmemb tulong) tint)
+              (Sset _t'2
+                (Ecast
+                  (Ebinop Olt (Ederef (Etempvar _child (tptr tint)) tint)
+                    (Ederef
+                      (Ebinop Oadd (Etempvar _child (tptr tint))
+                        (Econst_int (Int.repr 1) tint) (tptr tint)) tint)
+                    tint) tbool))
+              (Sset _t'2 (Econst_int (Int.repr 0) tint)))
+            (Sifthenelse (Etempvar _t'2 tint)
+              (Ssequence
+                (Sset _child
+                  (Ebinop Oadd (Etempvar _child (tptr tint))
+                    (Econst_int (Int.repr 1) tint) (tptr tint)))
+                (Sset _child_i
+                  (Ebinop Oadd (Etempvar _child_i tulong)
+                    (Econst_int (Int.repr 1) tint) tulong)))
+              Sskip))
+          (Ssequence
+            (Sset _par
+              (Ebinop Oadd (Etempvar _base (tptr tint))
+                (Etempvar _par_i tulong) (tptr tint)))
+            (Ssequence
+              (Sifthenelse (Ebinop Ole
+                             (Ederef (Etempvar _child (tptr tint)) tint)
+                             (Ederef (Etempvar _par (tptr tint)) tint) tint)
+                Sbreak
+                Sskip)
+              (Ssequence
+                (Sset _tmp (Ederef (Etempvar _par (tptr tint)) tint))
+                (Ssequence
+                  (Sassign (Ederef (Etempvar _par (tptr tint)) tint)
+                    (Ederef (Etempvar _child (tptr tint)) tint))
+                  (Sassign (Ederef (Etempvar _child (tptr tint)) tint)
+                    (Etempvar _tmp tint)))))))))
+    (Sset _par_i (Etempvar _child_i tulong))))
+|}.
+
+Definition f_heapify := {|
+  fn_return := tvoid;
+  fn_callconv := cc_default;
+  fn_params := ((_base, (tptr tint)) :: (_nmemb, tulong) :: (_k, tint) ::
+                nil);
+  fn_vars := nil;
+  fn_temps := ((_par_i, tulong) :: (_child_i, tulong) ::
+               (_par, (tptr tint)) :: (_child, (tptr tint)) ::
+               (_t'3, tint) :: (_t'2, tint) :: (_t'1, tulong) :: nil);
+  fn_body :=
+(Ssequence
+  (Ssequence
+    (Sset _par_i (Ecast (Econst_int (Int.repr 1) tint) tulong))
+    (Sloop
+      (Ssequence
+        (Ssequence
+          (Ssequence
+            (Sset _t'1
+              (Ecast
+                (Ebinop Omul (Etempvar _par_i tulong)
+                  (Econst_int (Int.repr 2) tint) tulong) tulong))
+            (Sset _child_i (Etempvar _t'1 tulong)))
+          (Sifthenelse (Ebinop Ole (Etempvar _t'1 tulong)
+                         (Etempvar _nmemb tulong) tint)
+            Sskip
+            Sbreak))
+        (Ssequence
+          (Sset _child
+            (Ebinop Oadd (Etempvar _base (tptr tint))
+              (Etempvar _child_i tulong) (tptr tint)))
+          (Ssequence
+            (Ssequence
+              (Sifthenelse (Ebinop Olt (Etempvar _child_i tulong)
+                             (Etempvar _nmemb tulong) tint)
+                (Sset _t'2
+                  (Ecast
+                    (Ebinop Olt (Ederef (Etempvar _child (tptr tint)) tint)
+                      (Ederef
+                        (Ebinop Oadd (Etempvar _child (tptr tint))
+                          (Econst_int (Int.repr 1) tint) (tptr tint)) tint)
+                      tint) tbool))
+                (Sset _t'2 (Econst_int (Int.repr 0) tint)))
+              (Sifthenelse (Etempvar _t'2 tint)
+                (Ssequence
+                  (Sset _child
+                    (Ebinop Oadd (Etempvar _child (tptr tint))
+                      (Econst_int (Int.repr 1) tint) (tptr tint)))
+                  (Sset _child_i
+                    (Ebinop Oadd (Etempvar _child_i tulong)
+                      (Econst_int (Int.repr 1) tint) tulong)))
+                Sskip))
+            (Ssequence
+              (Sset _par
+                (Ebinop Oadd (Etempvar _base (tptr tint))
+                  (Etempvar _par_i tulong) (tptr tint)))
+              (Sassign (Ederef (Etempvar _par (tptr tint)) tint)
+                (Ederef (Etempvar _child (tptr tint)) tint))))))
+      (Sset _par_i (Etempvar _child_i tulong))))
+  (Sloop
+    (Ssequence
+      Sskip
+      (Ssequence
+        (Sset _child_i (Etempvar _par_i tulong))
+        (Ssequence
+          (Sset _par_i
+            (Ebinop Odiv (Etempvar _child_i tulong)
+              (Econst_int (Int.repr 2) tint) tulong))
+          (Ssequence
+            (Sset _child
+              (Ebinop Oadd (Etempvar _base (tptr tint))
+                (Etempvar _child_i tulong) (tptr tint)))
+            (Ssequence
+              (Sset _par
+                (Ebinop Oadd (Etempvar _base (tptr tint))
+                  (Etempvar _par_i tulong) (tptr tint)))
+              (Ssequence
+                (Ssequence
+                  (Sifthenelse (Ebinop Oeq (Etempvar _child_i tulong)
+                                 (Econst_int (Int.repr 1) tint) tint)
+                    (Sset _t'3 (Econst_int (Int.repr 1) tint))
+                    (Sset _t'3
+                      (Ecast
+                        (Ebinop Olt (Etempvar _k tint)
+                          (Ederef (Etempvar _par (tptr tint)) tint) tint)
+                        tbool)))
+                  (Sifthenelse (Etempvar _t'3 tint)
+                    (Ssequence
+                      (Sassign (Ederef (Etempvar _child (tptr tint)) tint)
+                        (Etempvar _k tint))
+                      Sbreak)
+                    Sskip))
+                (Sassign (Ederef (Etempvar _child (tptr tint)) tint)
+                  (Ederef (Etempvar _par (tptr tint)) tint))))))))
+    Sskip))
+|}.
+
+Definition f_heapsort := {|
+  fn_return := tvoid;
+  fn_callconv := cc_default;
+  fn_params := ((_vbase, (tptr tint)) :: (_nmemb, tulong) :: nil);
+  fn_vars := nil;
+  fn_temps := ((_base, (tptr tint)) :: (_l, tulong) :: (_k, tint) ::
+               (_t'1, tulong) :: nil);
+  fn_body :=
+(Ssequence
+  (Sifthenelse (Ebinop Ole (Etempvar _nmemb tulong)
+                 (Econst_int (Int.repr 1) tint) tint)
+    (Sreturn None)
+    Sskip)
+  (Ssequence
+    (Sset _base
+      (Ebinop Osub (Etempvar _vbase (tptr tint))
+        (Econst_int (Int.repr 1) tint) (tptr tint)))
+    (Ssequence
+      (Ssequence
+        (Sset _l
+          (Ebinop Oadd
+            (Ebinop Odiv (Etempvar _nmemb tulong)
+              (Econst_int (Int.repr 2) tint) tulong)
+            (Econst_int (Int.repr 1) tint) tulong))
+        (Sloop
+          (Ssequence
+            (Ssequence
+              (Ssequence
+                (Sset _t'1
+                  (Ecast
+                    (Ebinop Osub (Etempvar _l tulong)
+                      (Econst_int (Int.repr 1) tint) tulong) tulong))
+                (Sset _l (Etempvar _t'1 tulong)))
+              (Sifthenelse (Etempvar _t'1 tulong) Sskip Sbreak))
+            (Scall None
+              (Evar _create (Tfunction
+                              (Tcons (tptr tint)
+                                (Tcons tulong (Tcons tulong Tnil))) tvoid
+                              cc_default))
+              ((Etempvar _base (tptr tint)) :: (Etempvar _nmemb tulong) ::
+               (Etempvar _l tulong) :: nil)))
+          Sskip))
+      (Swhile
+        (Ebinop Ogt (Etempvar _nmemb tulong) (Econst_int (Int.repr 1) tint)
+          tint)
+        (Ssequence
+          (Sset _k
+            (Ederef
+              (Ebinop Oadd (Etempvar _base (tptr tint))
+                (Etempvar _nmemb tulong) (tptr tint)) tint))
+          (Ssequence
+            (Sassign
+              (Ederef
+                (Ebinop Oadd (Etempvar _base (tptr tint))
+                  (Etempvar _nmemb tulong) (tptr tint)) tint)
+              (Ederef
+                (Ebinop Oadd (Etempvar _base (tptr tint))
+                  (Econst_int (Int.repr 1) tint) (tptr tint)) tint))
+            (Ssequence
+              (Sset _nmemb
+                (Ebinop Osub (Etempvar _nmemb tulong)
+                  (Econst_int (Int.repr 1) tint) tulong))
+              (Scall None
+                (Evar _heapify (Tfunction
+                                 (Tcons (tptr tint)
+                                   (Tcons tulong (Tcons tint Tnil))) tvoid
+                                 cc_default))
+                ((Etempvar _base (tptr tint)) :: (Etempvar _nmemb tulong) ::
+                 (Etempvar _k tint) :: nil)))))))))
+|}.
+
+Definition composites : list composite_definition :=
+nil.
+
+Definition global_definitions : list (ident * globdef fundef type) :=
+((___compcert_va_int32,
+   Gfun(External (EF_runtime "__compcert_va_int32"
+                   (mksignature (AST.Tlong :: nil) AST.Tint cc_default))
+     (Tcons (tptr tvoid) Tnil) tuint cc_default)) ::
+ (___compcert_va_int64,
+   Gfun(External (EF_runtime "__compcert_va_int64"
+                   (mksignature (AST.Tlong :: nil) AST.Tlong cc_default))
+     (Tcons (tptr tvoid) Tnil) tulong cc_default)) ::
+ (___compcert_va_float64,
+   Gfun(External (EF_runtime "__compcert_va_float64"
+                   (mksignature (AST.Tlong :: nil) AST.Tfloat cc_default))
+     (Tcons (tptr tvoid) Tnil) tdouble cc_default)) ::
+ (___compcert_va_composite,
+   Gfun(External (EF_runtime "__compcert_va_composite"
+                   (mksignature (AST.Tlong :: AST.Tlong :: nil) AST.Tlong
+                     cc_default)) (Tcons (tptr tvoid) (Tcons tulong Tnil))
+     (tptr tvoid) cc_default)) ::
+ (___compcert_i64_dtos,
+   Gfun(External (EF_runtime "__compcert_i64_dtos"
+                   (mksignature (AST.Tfloat :: nil) AST.Tlong cc_default))
+     (Tcons tdouble Tnil) tlong cc_default)) ::
+ (___compcert_i64_dtou,
+   Gfun(External (EF_runtime "__compcert_i64_dtou"
+                   (mksignature (AST.Tfloat :: nil) AST.Tlong cc_default))
+     (Tcons tdouble Tnil) tulong cc_default)) ::
+ (___compcert_i64_stod,
+   Gfun(External (EF_runtime "__compcert_i64_stod"
+                   (mksignature (AST.Tlong :: nil) AST.Tfloat cc_default))
+     (Tcons tlong Tnil) tdouble cc_default)) ::
+ (___compcert_i64_utod,
+   Gfun(External (EF_runtime "__compcert_i64_utod"
+                   (mksignature (AST.Tlong :: nil) AST.Tfloat cc_default))
+     (Tcons tulong Tnil) tdouble cc_default)) ::
+ (___compcert_i64_stof,
+   Gfun(External (EF_runtime "__compcert_i64_stof"
+                   (mksignature (AST.Tlong :: nil) AST.Tsingle cc_default))
+     (Tcons tlong Tnil) tfloat cc_default)) ::
+ (___compcert_i64_utof,
+   Gfun(External (EF_runtime "__compcert_i64_utof"
+                   (mksignature (AST.Tlong :: nil) AST.Tsingle cc_default))
+     (Tcons tulong Tnil) tfloat cc_default)) ::
+ (___compcert_i64_sdiv,
+   Gfun(External (EF_runtime "__compcert_i64_sdiv"
+                   (mksignature (AST.Tlong :: AST.Tlong :: nil) AST.Tlong
+                     cc_default)) (Tcons tlong (Tcons tlong Tnil)) tlong
+     cc_default)) ::
+ (___compcert_i64_udiv,
+   Gfun(External (EF_runtime "__compcert_i64_udiv"
+                   (mksignature (AST.Tlong :: AST.Tlong :: nil) AST.Tlong
+                     cc_default)) (Tcons tulong (Tcons tulong Tnil)) tulong
+     cc_default)) ::
+ (___compcert_i64_smod,
+   Gfun(External (EF_runtime "__compcert_i64_smod"
+                   (mksignature (AST.Tlong :: AST.Tlong :: nil) AST.Tlong
+                     cc_default)) (Tcons tlong (Tcons tlong Tnil)) tlong
+     cc_default)) ::
+ (___compcert_i64_umod,
+   Gfun(External (EF_runtime "__compcert_i64_umod"
+                   (mksignature (AST.Tlong :: AST.Tlong :: nil) AST.Tlong
+                     cc_default)) (Tcons tulong (Tcons tulong Tnil)) tulong
+     cc_default)) ::
+ (___compcert_i64_shl,
+   Gfun(External (EF_runtime "__compcert_i64_shl"
+                   (mksignature (AST.Tlong :: AST.Tint :: nil) AST.Tlong
+                     cc_default)) (Tcons tlong (Tcons tint Tnil)) tlong
+     cc_default)) ::
+ (___compcert_i64_shr,
+   Gfun(External (EF_runtime "__compcert_i64_shr"
+                   (mksignature (AST.Tlong :: AST.Tint :: nil) AST.Tlong
+                     cc_default)) (Tcons tulong (Tcons tint Tnil)) tulong
+     cc_default)) ::
+ (___compcert_i64_sar,
+   Gfun(External (EF_runtime "__compcert_i64_sar"
+                   (mksignature (AST.Tlong :: AST.Tint :: nil) AST.Tlong
+                     cc_default)) (Tcons tlong (Tcons tint Tnil)) tlong
+     cc_default)) ::
+ (___compcert_i64_smulh,
+   Gfun(External (EF_runtime "__compcert_i64_smulh"
+                   (mksignature (AST.Tlong :: AST.Tlong :: nil) AST.Tlong
+                     cc_default)) (Tcons tlong (Tcons tlong Tnil)) tlong
+     cc_default)) ::
+ (___compcert_i64_umulh,
+   Gfun(External (EF_runtime "__compcert_i64_umulh"
+                   (mksignature (AST.Tlong :: AST.Tlong :: nil) AST.Tlong
+                     cc_default)) (Tcons tulong (Tcons tulong Tnil)) tulong
+     cc_default)) ::
+ (___builtin_ais_annot,
+   Gfun(External (EF_builtin "__builtin_ais_annot"
+                   (mksignature (AST.Tlong :: nil) AST.Tvoid
+                     {|cc_vararg:=(Some 1); cc_unproto:=false; cc_structret:=false|}))
+     (Tcons (tptr tschar) Tnil) tvoid
+     {|cc_vararg:=(Some 1); cc_unproto:=false; cc_structret:=false|})) ::
+ (___builtin_bswap64,
+   Gfun(External (EF_builtin "__builtin_bswap64"
+                   (mksignature (AST.Tlong :: nil) AST.Tlong cc_default))
+     (Tcons tulong Tnil) tulong cc_default)) ::
+ (___builtin_bswap,
+   Gfun(External (EF_builtin "__builtin_bswap"
+                   (mksignature (AST.Tint :: nil) AST.Tint cc_default))
+     (Tcons tuint Tnil) tuint cc_default)) ::
+ (___builtin_bswap32,
+   Gfun(External (EF_builtin "__builtin_bswap32"
+                   (mksignature (AST.Tint :: nil) AST.Tint cc_default))
+     (Tcons tuint Tnil) tuint cc_default)) ::
+ (___builtin_bswap16,
+   Gfun(External (EF_builtin "__builtin_bswap16"
+                   (mksignature (AST.Tint :: nil) AST.Tint16unsigned
+                     cc_default)) (Tcons tushort Tnil) tushort cc_default)) ::
+ (___builtin_clz,
+   Gfun(External (EF_builtin "__builtin_clz"
+                   (mksignature (AST.Tint :: nil) AST.Tint cc_default))
+     (Tcons tuint Tnil) tint cc_default)) ::
+ (___builtin_clzl,
+   Gfun(External (EF_builtin "__builtin_clzl"
+                   (mksignature (AST.Tlong :: nil) AST.Tint cc_default))
+     (Tcons tulong Tnil) tint cc_default)) ::
+ (___builtin_clzll,
+   Gfun(External (EF_builtin "__builtin_clzll"
+                   (mksignature (AST.Tlong :: nil) AST.Tint cc_default))
+     (Tcons tulong Tnil) tint cc_default)) ::
+ (___builtin_ctz,
+   Gfun(External (EF_builtin "__builtin_ctz"
+                   (mksignature (AST.Tint :: nil) AST.Tint cc_default))
+     (Tcons tuint Tnil) tint cc_default)) ::
+ (___builtin_ctzl,
+   Gfun(External (EF_builtin "__builtin_ctzl"
+                   (mksignature (AST.Tlong :: nil) AST.Tint cc_default))
+     (Tcons tulong Tnil) tint cc_default)) ::
+ (___builtin_ctzll,
+   Gfun(External (EF_builtin "__builtin_ctzll"
+                   (mksignature (AST.Tlong :: nil) AST.Tint cc_default))
+     (Tcons tulong Tnil) tint cc_default)) ::
+ (___builtin_fabs,
+   Gfun(External (EF_builtin "__builtin_fabs"
+                   (mksignature (AST.Tfloat :: nil) AST.Tfloat cc_default))
+     (Tcons tdouble Tnil) tdouble cc_default)) ::
+ (___builtin_fabsf,
+   Gfun(External (EF_builtin "__builtin_fabsf"
+                   (mksignature (AST.Tsingle :: nil) AST.Tsingle cc_default))
+     (Tcons tfloat Tnil) tfloat cc_default)) ::
+ (___builtin_fsqrt,
+   Gfun(External (EF_builtin "__builtin_fsqrt"
+                   (mksignature (AST.Tfloat :: nil) AST.Tfloat cc_default))
+     (Tcons tdouble Tnil) tdouble cc_default)) ::
+ (___builtin_sqrt,
+   Gfun(External (EF_builtin "__builtin_sqrt"
+                   (mksignature (AST.Tfloat :: nil) AST.Tfloat cc_default))
+     (Tcons tdouble Tnil) tdouble cc_default)) ::
+ (___builtin_memcpy_aligned,
+   Gfun(External (EF_builtin "__builtin_memcpy_aligned"
+                   (mksignature
+                     (AST.Tlong :: AST.Tlong :: AST.Tlong :: AST.Tlong ::
+                      nil) AST.Tvoid cc_default))
+     (Tcons (tptr tvoid)
+       (Tcons (tptr tvoid) (Tcons tulong (Tcons tulong Tnil)))) tvoid
+     cc_default)) ::
+ (___builtin_sel,
+   Gfun(External (EF_builtin "__builtin_sel"
+                   (mksignature (AST.Tint :: nil) AST.Tvoid
+                     {|cc_vararg:=(Some 1); cc_unproto:=false; cc_structret:=false|}))
+     (Tcons tbool Tnil) tvoid
+     {|cc_vararg:=(Some 1); cc_unproto:=false; cc_structret:=false|})) ::
+ (___builtin_annot,
+   Gfun(External (EF_builtin "__builtin_annot"
+                   (mksignature (AST.Tlong :: nil) AST.Tvoid
+                     {|cc_vararg:=(Some 1); cc_unproto:=false; cc_structret:=false|}))
+     (Tcons (tptr tschar) Tnil) tvoid
+     {|cc_vararg:=(Some 1); cc_unproto:=false; cc_structret:=false|})) ::
+ (___builtin_annot_intval,
+   Gfun(External (EF_builtin "__builtin_annot_intval"
+                   (mksignature (AST.Tlong :: AST.Tint :: nil) AST.Tint
+                     cc_default)) (Tcons (tptr tschar) (Tcons tint Tnil))
+     tint cc_default)) ::
+ (___builtin_membar,
+   Gfun(External (EF_builtin "__builtin_membar"
+                   (mksignature nil AST.Tvoid cc_default)) Tnil tvoid
+     cc_default)) ::
+ (___builtin_va_start,
+   Gfun(External (EF_builtin "__builtin_va_start"
+                   (mksignature (AST.Tlong :: nil) AST.Tvoid cc_default))
+     (Tcons (tptr tvoid) Tnil) tvoid cc_default)) ::
+ (___builtin_va_arg,
+   Gfun(External (EF_builtin "__builtin_va_arg"
+                   (mksignature (AST.Tlong :: AST.Tint :: nil) AST.Tvoid
+                     cc_default)) (Tcons (tptr tvoid) (Tcons tuint Tnil))
+     tvoid cc_default)) ::
+ (___builtin_va_copy,
+   Gfun(External (EF_builtin "__builtin_va_copy"
+                   (mksignature (AST.Tlong :: AST.Tlong :: nil) AST.Tvoid
+                     cc_default))
+     (Tcons (tptr tvoid) (Tcons (tptr tvoid) Tnil)) tvoid cc_default)) ::
+ (___builtin_va_end,
+   Gfun(External (EF_builtin "__builtin_va_end"
+                   (mksignature (AST.Tlong :: nil) AST.Tvoid cc_default))
+     (Tcons (tptr tvoid) Tnil) tvoid cc_default)) ::
+ (___builtin_unreachable,
+   Gfun(External (EF_builtin "__builtin_unreachable"
+                   (mksignature nil AST.Tvoid cc_default)) Tnil tvoid
+     cc_default)) ::
+ (___builtin_expect,
+   Gfun(External (EF_builtin "__builtin_expect"
+                   (mksignature (AST.Tlong :: AST.Tlong :: nil) AST.Tlong
+                     cc_default)) (Tcons tlong (Tcons tlong Tnil)) tlong
+     cc_default)) ::
+ (___builtin_fmax,
+   Gfun(External (EF_builtin "__builtin_fmax"
+                   (mksignature (AST.Tfloat :: AST.Tfloat :: nil) AST.Tfloat
+                     cc_default)) (Tcons tdouble (Tcons tdouble Tnil))
+     tdouble cc_default)) ::
+ (___builtin_fmin,
+   Gfun(External (EF_builtin "__builtin_fmin"
+                   (mksignature (AST.Tfloat :: AST.Tfloat :: nil) AST.Tfloat
+                     cc_default)) (Tcons tdouble (Tcons tdouble Tnil))
+     tdouble cc_default)) ::
+ (___builtin_fmadd,
+   Gfun(External (EF_builtin "__builtin_fmadd"
+                   (mksignature
+                     (AST.Tfloat :: AST.Tfloat :: AST.Tfloat :: nil)
+                     AST.Tfloat cc_default))
+     (Tcons tdouble (Tcons tdouble (Tcons tdouble Tnil))) tdouble
+     cc_default)) ::
+ (___builtin_fmsub,
+   Gfun(External (EF_builtin "__builtin_fmsub"
+                   (mksignature
+                     (AST.Tfloat :: AST.Tfloat :: AST.Tfloat :: nil)
+                     AST.Tfloat cc_default))
+     (Tcons tdouble (Tcons tdouble (Tcons tdouble Tnil))) tdouble
+     cc_default)) ::
+ (___builtin_fnmadd,
+   Gfun(External (EF_builtin "__builtin_fnmadd"
+                   (mksignature
+                     (AST.Tfloat :: AST.Tfloat :: AST.Tfloat :: nil)
+                     AST.Tfloat cc_default))
+     (Tcons tdouble (Tcons tdouble (Tcons tdouble Tnil))) tdouble
+     cc_default)) ::
+ (___builtin_fnmsub,
+   Gfun(External (EF_builtin "__builtin_fnmsub"
+                   (mksignature
+                     (AST.Tfloat :: AST.Tfloat :: AST.Tfloat :: nil)
+                     AST.Tfloat cc_default))
+     (Tcons tdouble (Tcons tdouble (Tcons tdouble Tnil))) tdouble
+     cc_default)) ::
+ (___builtin_read16_reversed,
+   Gfun(External (EF_builtin "__builtin_read16_reversed"
+                   (mksignature (AST.Tlong :: nil) AST.Tint16unsigned
+                     cc_default)) (Tcons (tptr tushort) Tnil) tushort
+     cc_default)) ::
+ (___builtin_read32_reversed,
+   Gfun(External (EF_builtin "__builtin_read32_reversed"
+                   (mksignature (AST.Tlong :: nil) AST.Tint cc_default))
+     (Tcons (tptr tuint) Tnil) tuint cc_default)) ::
+ (___builtin_write16_reversed,
+   Gfun(External (EF_builtin "__builtin_write16_reversed"
+                   (mksignature (AST.Tlong :: AST.Tint :: nil) AST.Tvoid
+                     cc_default)) (Tcons (tptr tushort) (Tcons tushort Tnil))
+     tvoid cc_default)) ::
+ (___builtin_write32_reversed,
+   Gfun(External (EF_builtin "__builtin_write32_reversed"
+                   (mksignature (AST.Tlong :: AST.Tint :: nil) AST.Tvoid
+                     cc_default)) (Tcons (tptr tuint) (Tcons tuint Tnil))
+     tvoid cc_default)) ::
+ (___builtin_debug,
+   Gfun(External (EF_external "__builtin_debug"
+                   (mksignature (AST.Tint :: nil) AST.Tvoid
+                     {|cc_vararg:=(Some 1); cc_unproto:=false; cc_structret:=false|}))
+     (Tcons tint Tnil) tvoid
+     {|cc_vararg:=(Some 1); cc_unproto:=false; cc_structret:=false|})) ::
+ (_create, Gfun(Internal f_create)) ::
+ (_heapify, Gfun(Internal f_heapify)) ::
+ (_heapsort, Gfun(Internal f_heapsort)) :: nil).
+
+Definition public_idents : list ident :=
+(_heapsort :: _heapify :: _create :: ___builtin_debug ::
+ ___builtin_write32_reversed :: ___builtin_write16_reversed ::
+ ___builtin_read32_reversed :: ___builtin_read16_reversed ::
+ ___builtin_fnmsub :: ___builtin_fnmadd :: ___builtin_fmsub ::
+ ___builtin_fmadd :: ___builtin_fmin :: ___builtin_fmax ::
+ ___builtin_expect :: ___builtin_unreachable :: ___builtin_va_end ::
+ ___builtin_va_copy :: ___builtin_va_arg :: ___builtin_va_start ::
+ ___builtin_membar :: ___builtin_annot_intval :: ___builtin_annot ::
+ ___builtin_sel :: ___builtin_memcpy_aligned :: ___builtin_sqrt ::
+ ___builtin_fsqrt :: ___builtin_fabsf :: ___builtin_fabs ::
+ ___builtin_ctzll :: ___builtin_ctzl :: ___builtin_ctz :: ___builtin_clzll ::
+ ___builtin_clzl :: ___builtin_clz :: ___builtin_bswap16 ::
+ ___builtin_bswap32 :: ___builtin_bswap :: ___builtin_bswap64 ::
+ ___builtin_ais_annot :: ___compcert_i64_umulh :: ___compcert_i64_smulh ::
+ ___compcert_i64_sar :: ___compcert_i64_shr :: ___compcert_i64_shl ::
+ ___compcert_i64_umod :: ___compcert_i64_smod :: ___compcert_i64_udiv ::
+ ___compcert_i64_sdiv :: ___compcert_i64_utof :: ___compcert_i64_stof ::
+ ___compcert_i64_utod :: ___compcert_i64_stod :: ___compcert_i64_dtou ::
+ ___compcert_i64_dtos :: ___compcert_va_composite ::
+ ___compcert_va_float64 :: ___compcert_va_int64 :: ___compcert_va_int32 ::
+ nil).
+
+Definition prog : Clight.program := 
+  mkprogram composites global_definitions public_idents _main Logic.I.
+
+
